dllbc/Dllbc.lean
@@ -10,6 +10,8 @@ import Dllbc.PureMacro
 import Dllbc.StdLemmas
 import Dllbc.DeclMacro
 import Dllbc.AlphaEq
+import Dllbc.Program
+import Dllbc.ProgMacro
 import Dllbc.Tests.S2
 import Dllbc.Tests.S3
 import Dllbc.Tests.S3Sym
@@ -34,6 +36,7 @@ import Dllbc.Tests.S26Seal
 import Dllbc.Tests.S26Modes
 import Dllbc.Tests.S26Rec
 import Dllbc.Tests.S26Fn
+import Dllbc.Tests.S26Prog
 import Dllbc.Tests.SInternals
 import Dllbc.Tests.SDeclMacro
 import Dllbc.Tests.SDeclMacroCrown
